%%% Template originaly created by Karol Kozio≈Ç (mail@karol-koziol.net) and modified for ShareLaTeX use

\documentclass[a4paper,11pt,fleqn]{article}

\usepackage[T1]{fontenc}
\usepackage[utf8]{inputenc}
\usepackage{graphicx}
\usepackage{xcolor}

\usepackage{tgtermes}
\usepackage{bussproofs}
\usepackage{blindtext}

\usepackage[
pdftitle={CMPS 242-HM2}, 
pdfauthor={jianfeng},
colorlinks=true,linkcolor=blue,urlcolor=blue,citecolor=blue,bookmarks=true,
bookmarksopenlevel=2]{hyperref}
\usepackage{amsmath,amssymb,amsthm,textcomp}
\usepackage{enumerate}
\usepackage{multicol}
\usepackage{tikz}

\usepackage{geometry}
\geometry{total={210mm,297mm},
left=25mm,right=25mm,%
bindingoffset=0mm, top=20mm,bottom=20mm}


\linespread{1.3}

\newcommand{\linia}{\rule{\linewidth}{0.5pt}}

% custom theorems if needed
\newtheoremstyle{mytheor}
    {1ex}{1ex}{\normalfont}{0pt}{\scshape}{.}{1ex}
    {{\thmname{#1 }}{\thmnumber{#2}}{\thmnote{ (#3)}}}

\theoremstyle{mytheor}
\newtheorem{defi}{Definition}

% my own titles
\makeatletter
\renewcommand{\maketitle}{
\begin{center}
\vspace{2ex}
{\huge \textsc{\@title}}
\vspace{1ex}
\\
\linia\\
\@author \hfill \@date
\vspace{4ex}
\end{center}
}
\makeatother
%%%

% custom footers and headers
\usepackage{fancyhdr,lastpage}
\pagestyle{fancy}
\lhead{}
\chead{}
\rhead{}
\lfoot{JIANFENG ZHAO}
\cfoot{ \thepage}
\rfoot{HM3}
\renewcommand{\headrulewidth}{0pt}
\renewcommand{\footrulewidth}{0pt}
%

%%%----------%%%----------%%%----------%%%----------%%%

\begin{document}

\title{CMPS 203 -- HM3}

\author{NAME: Jianfeng Zhao, CruzID: jzhao65}

\date{25/04/2018}

\maketitle




\subsection*{Quetiion 1}
$Question.$ In the $\mathrm{WHILE}$ language, prove or disprove the equivalence of the two commands:\\
$$\mathrm{t} := \mathrm{x};\mathrm{x} := \mathrm{y};\mathrm{y} := \mathrm{t};$$
and\\
$$\mathrm{t} := \mathrm{y};\mathrm{y} := \mathrm{x};\mathrm{x} := \mathrm{t};$$
$Proof.$ we define the first commands as $\mathrm{C}_1$ and the second commands as $\mathrm{C}_2$. Hence, the two commands are equivalence only if \\
$$\langle \mathrm{C}_1, s \rangle \to s' and\  \langle \mathrm{c}_2, s \rangle \to s'$$
However, we assume $s$ is $s[t: t_0, x: x_0, y: y_0]$.\\
It easy to get the first commands $\langle \mathrm{C}_1, s \rangle  \to s'[t:x_0, x: y_0, y: x_0]$.\\
But the second commands' state is $\langle \mathrm{C}_2, s \rangle  \to s''[t:y_0, x: y_0, y: x_0]$.\\
Hence, $s' \ne s'' \Rightarrow \mathrm{C_1} \ne \mathrm{C_2}$\\
As a result, we disprove the semanticlly equivalent of these two commands. \\

\subsection*{Quetiion 2}
$Question.$ In the $\mathrm{WHILE}$ , prove that if\\
$$ \langle \mathrm{while\ b\ do\ y} := \mathrm{y} - \mathrm{x}, \mathrm{s} \rangle \ \Downarrow \mathrm{s'}$$
then there exists an integer $k$ such that\\
$$s(y) = s'(y) + k\ *\ s(x)$$
Please make it explicit if/when you reason by induction on derivations, stating your induction hypothesis.\\
\\
$Proof.$ We assume the command always terminate. we prove the command with induction.\\
\\
\begin{itemize}
\item Base Case: $p(0)$ means this while run zero times. we have
\begin{prooftree}
	\AxiomC{$\langle b, s \rangle \Downarrow \mathrm{false}$}
	\AxiomC{$\langle skip, s \rangle \Downarrow \ s'$}
	\BinaryInfC{$\langle \mathrm{while\ b\ do\ y}\ :=\ \mathrm{y\ -\ x}, s \rangle \Downarrow s'$}
\end{prooftree}
It's easy to see $s(y) = s'(y) + 0 \times s(x)$\\
\\
\item We assume p(n) means while run n loops and we have
$$ s(y) = s'(y) + n \times s(x)$$
We need to prove $p(n + 1)$ which is $\langle while\ b\ do\ y\ :=\ y\ -\ x, s \rangle \Downarrow s'$ we have
$$ s(y) = s''(y) + (n + 1) \times s(x)$$
\item We can build the derivation tree as blow
\begin{prooftree}
	\AxiomC{$\langle b, s \rangle \Downarrow \mathrm{true}$}
	\AxiomC{$\langle \mathrm{while\ b\ do\ y}\ :=\ \mathrm{y\ -\ x}, s \rangle \Downarrow s'$}
	\AxiomC{$\langle \mathrm{y := y\ - \ x}, s' \rangle \Downarrow s''$}
	\TrinaryInfC{$\langle \mathrm{while\ b\ do\ y}\ :=\ \mathrm{y\ -\ x}, s' \rangle \Downarrow s''$}
\end{prooftree}
by induction hypothiesi, we know that\\
$$s(y) = s'(y) + n \times s(x)$$
we also know the derivation tree about $p(n + 1)$ that
$$s'(y) = s''(y) + s(x)$$
Because of $\langle \mathrm{y := y\ - \ x}, s' \rangle \Downarrow s''$, Hence, we have
\begin{equation}
\begin{split}
s(y) &= s'(y) + n \times s(x)\\
&= s''(y) + x + n\times s(x)\\
&= s''(y) + (n + 1) \times s(x)
\nonumber
\end{split}
\end{equation}
\end{itemize}
Hence, the statement is proved. 
\subsection*{Quetiion 3}
$Question.$ In the $\mathrm{WHILE}$ , prove 
$$\forall c_1, c_2, c_3\  .\ c_1;(c_2;c_3)\ \approx \ (c_1;c_2);c_3$$
\\
$Prove.$ We assume 
$$\langle c_1, s_0 \rangle \Downarrow s_1$$
$$\langle c_2, s_1 \rangle \Downarrow s_2$$
$$\langle c_3, s_2 \rangle \Downarrow s_3$$
We have derivation tree of right part. 
\begin{prooftree}
	\AxiomC{$\langle c_1, s_0 \rangle \Downarrow s_1$}
	\AxiomC{$\langle c_2, s_1 \rangle \Downarrow s_2$}
	\BinaryInfC{$\langle c_1;c_2, s_0 \rangle \Downarrow s_2$}
	\AxiomC{$\langle c_3, s_2 \rangle \Downarrow s_3$}
	\BinaryInfC{$\langle (c_1;c_2);c_3,s_0 \rangle \Downarrow s_3$}
\end{prooftree}
derivation tree of left part.
\begin{prooftree}
	\AxiomC{$\langle c_1, s_0 \rangle \Downarrow s_1$}
	\AxiomC{$\langle c_2, s_1 \rangle \Downarrow s_2$}
	\AxiomC{$\langle c_3, s_2 \rangle \Downarrow s_3$}
	\BinaryInfC{$\langle c_2;c_3, s_1 \rangle \Downarrow s_3$}
	\BinaryInfC{$\langle c_1;(c_2;c_3),s_0 \rangle \Downarrow s_3$}
\end{prooftree}
Hence we have 
$$\langle (c_1;c_2);c_3, s_0 \rangle \Downarrow s_3$$
$$\langle c_1;(c_2;c_3), s_0 \rangle \Downarrow s_3$$
Hence, we prove that 
$$\forall c_1, c_2, c_3\  .\ c_1;(c_2;c_3)\ \approx \ (c_1;c_2);c_3$$
\end{document}
