%%% Template originaly created by Karol Kozioł (mail@karol-koziol.net) and modified for ShareLaTeX use

\documentclass[a4paper,11pt,fleqn]{article}

\usepackage[T1]{fontenc}
\usepackage[utf8]{inputenc}
\usepackage{graphicx}
\usepackage{xcolor}

\usepackage{tgtermes}
\usepackage{bussproofs}
\usepackage{blindtext}

\usepackage[
pdftitle={CMPS 203-HM5}, 
pdfauthor={jianfeng},
colorlinks=true,linkcolor=blue,urlcolor=blue,citecolor=blue,bookmarks=true,
bookmarksopenlevel=2]{hyperref}
\usepackage{amsmath,amssymb,amsthm,textcomp}
\usepackage{enumerate}
\usepackage{multicol}
\usepackage{tikz}

\usepackage{geometry}
\geometry{total={210mm,297mm},
left=25mm,right=25mm,%
bindingoffset=0mm, top=20mm,bottom=20mm}


\linespread{1.3}

\newcommand{\linia}{\rule{\linewidth}{0.5pt}}

% custom theorems if needed
\newtheoremstyle{mytheor}
    {1ex}{1ex}{\normalfont}{0pt}{\scshape}{.}{1ex}
    {{\thmname{#1 }}{\thmnumber{#2}}{\thmnote{ (#3)}}}

\theoremstyle{mytheor}
\newtheorem{defi}{Definition}

% my own titles
\makeatletter
\renewcommand{\maketitle}{
\begin{center}
\vspace{2ex}
{\huge \textsc{\@title}}
\vspace{1ex}
\\
\linia\\
\@author \hfill \@date
\vspace{4ex}
\end{center}
}
\makeatother
%%%

% custom footers and headers
\usepackage{fancyhdr,lastpage}
\pagestyle{fancy}
\lhead{}
\chead{}
\rhead{}
\lfoot{JIANFENG ZHAO}
\cfoot{ \thepage}
\rfoot{HM5}
\renewcommand{\headrulewidth}{0pt}
\renewcommand{\footrulewidth}{0pt}
%

%%%----------%%%----------%%%----------%%%----------%%%
\def\changemargin#1#2{\list{}{\rightmargin#2\leftmargin#1}\item[]}
\let\endchangemargin=\endlist 
\begin{document}

\title{CMPS 203 -- HM5}

\author{NAME: Jianfeng Zhao, CruzID: jzhao65}

\date{10/05/2018}

\maketitle




\section*{$Quetiion 1.$}
Using Hoare’s rules, prove:
$$\{ x = y \}\ x:=x+1;\ y:=y+1\ \{x=y\}  $$
$Proof.$ We can get this by Sequence Rule and Assign Rule.
\begin{prooftree}
	\AxiomC{$x=y \Rightarrow x + 1 = y + 1$}
	\AxiomC{$\{x + 1 = y + 1\}x:=x+1\{x = y + 1\}$}
	\AxiomC{$\{x = y + 1\}y:=y+1\{x = y\}$}
	\BinaryInfC{$\{x+1=y+1\}\ x:=x+1;\ y:=y+1\ \{x=y\}$}
	\BinaryInfC{$\{ x = y \}\ x:=x+1;\ y:=y+1\ \{x=y\}$}
\end{prooftree}
\section*{$Quetiion 2.$}
Using Hoare’s rules, prove:
$$\{y=z\}while\ b\ do\ y:=y-x\ \{\exists k.z=(y+k*x) \}$$
for an arbitrary boolean expression b.\\
$Proof.$ 
\begin{itemize}
\item(1) For the Precondition, It's easy to proof by Consequence Rule\\
\begin{prooftree}
	\AxiomC{\{$y = z\} \Rightarrow \{z = y + 0 * x\}$}
	\AxiomC{$\{z = y + 0 * x\} \Rightarrow \{\exists k.z=(y+k*x)\} $}
	\BinaryInfC{$\{y = z\} \Rightarrow \{\exists k.z=(y+k*x)\}$}
\end{prooftree}
\item(2) Otherwise, we can get below by Assign Rule and Sequence Rule.\\
\begin{changemargin}{-1cm}{0cm}
\begin{prooftree}
	\AxiomC{$\{\exists k.z = y - x + k * x\} \Rightarrow \{\exists k.z = y + (k-1) * x\} $}
	\AxiomC{$\{\exists k.z = y - x + k * x\} y:=y - x \{\exists k. z = y + k * x\}$}
	\BinaryInfC{$\{\exists k.z = y + (k-1) * x\} y:=y - x\{\exists k. z = (y + k * x)\}$}
\end{prooftree}
\begin{prooftree}
	\AxiomC{$\{\exists k.z = y + (k-1) * x\} \Rightarrow \{\exists k.z = y + k * x\} $}
	\AxiomC{$\{\exists k.z = y + (k-1) * x\} y:=y - x \{\exists k. z = y + k * x\}$}
	\BinaryInfC{$\{\exists k.z = (y + k * x)\} y:=y - x\{\exists k. z = (y + k * x)\}$}
\end{prooftree}
\end{changemargin}
\item(3) From (1) and (2) and While Loop Rule and Consequence Rule, we can get\\
\begin{prooftree}
\AxiomC{$\{y = z\} \Rightarrow \{\exists k.z=(y+k*x)\}$}
\AxiomC{$\{\exists k.z = (y + k * x)\} y:=y - x \{\exists k.z=(y+k*x)\}$}
\BinaryInfC{$\{y = z\}y:=y - x \{\exists k.z=(y+k*x)\}$}
\UnaryInfC{$\{y=z\}while\ b\ do\ y:=y-x\ \{\exists k.z=(y+k*x) \}$}
\end{prooftree}
\end{itemize}
Hence, $\{y=z\}while\ b\ do\ y:=y-x\ \{\exists k.z=(y+k*x) \}$. for an arbitrary boolean expression b.\\


\end{document}
